Rename from False to Void

syntax.sig
@@ -4,9 +4,9 @@ nat : Type
 tAbs : tm -> (tm -> tm) -> tm
 tApp : tm -> tm -> tm
 tPi : tm -> (tm -> tm) -> tm
-tFalse : tm
+tVoid : tm
 tUniv : nat -> tm
-tOn : tm
-tOff : tm
+tTrue : tm
+tFalse : tm
 tIf : tm -> tm -> tm -> tm
-tSwitch : tm
+tBool : tm
